PosWrapper.v
@@ -3,6 +3,7 @@ From Stdlib Require Import ZArith.
 Class PosWrapper (A : Type) := {
   wrap   : positive -> A;
   unwrap : A -> positive;
+  incr   : A -> A;
 }.
 
 From MyProject Require Import CrIdentifiers.
@@ -10,28 +11,35 @@ From MyProject Require Import CrIdentifiers.
 Instance PosWrapper_ParserState : PosWrapper ParserState := {
   wrap := fun p => ParserStateCtr p;
   unwrap := fun s => match s with ParserStateCtr p => p end;
+  incr := fun s => match s with ParserStateCtr p => ParserStateCtr (p + 1) end
 }.
 Instance PosWrapper_Header : PosWrapper Header := {
   wrap := fun p => HeaderCtr p;
   unwrap := fun s => match s with HeaderCtr p => p end;
+  incr := fun s => match s with HeaderCtr p => HeaderCtr (p + 1) end;
 }.
 Instance PosWrapper_State : PosWrapper State := {
   wrap := fun p => StateCtr p;
   unwrap := fun s => match s with StateCtr p => p end;
+  incr := fun s => match s with StateCtr p => StateCtr (p + 1) end;
 }.
 Instance PosWrapper_ModuleName : PosWrapper ModuleName := {
   wrap := fun p => ModuleNameCtr p;
   unwrap := fun s => match s with ModuleNameCtr p => p end;
+  incr := fun s => match s with ModuleNameCtr p => ModuleNameCtr (p + 1) end;
 }.
 Instance PosWrapper_FunctionName : PosWrapper FunctionName := {
   wrap := fun p => FunctionNameCtr p;
   unwrap := fun s => match s with FunctionNameCtr p => p end;
+  incr := fun s => match s with FunctionNameCtr p => FunctionNameCtr (p + 1) end;
 }.
 Instance PosWrapper_ConnectionName: PosWrapper ConnectionName := {
   wrap := fun p => ConnectionNameCtr p;
   unwrap := fun s => match s with ConnectionNameCtr p => p end;
+  incr := fun s => match s with ConnectionNameCtr p => ConnectionNameCtr (p + 1) end;
 }.
 Instance PosWrapper_Ctrl : PosWrapper Ctrl := {
   wrap := fun p => CtrlCtr p;
   unwrap := fun s => match s with CtrlCtr p => p end;
+  incr := fun s => match s with CtrlCtr p => CtrlCtr (p + 1) end;
 }.
